\documentclass[UTF8]{ctexart}
\usepackage{amsmath}

\begin{document}
\begin{enumerate}
\item \begin{itemize}
\item[(a)] 
\begin{align*}
\frac{1 - \sec x}{\tan^2x} &= \frac{1 - \frac{1}{\cos x}}{\frac{\sin^2 x}{\cos^2 x}} \\
&= \frac{\cos^2 x - \cos x}{\sin^2 x} \\
&= -\frac{\cos x(\cos x - 1)}{\cos^2 x - 1} \\
&= -\frac{\cos x(\cos x - 1)}{(\cos x - 1)(\cos x + 1)} \\
&= -\frac{\cos x}{\cos x + 1} \\
&= -\frac{1}{1 + \sec x}
\end{align*}
When $x$ is near $2\pi n$, there is subtraction of nearly equal numbers.

\item[(b)] 
\begin{align*}
\frac{1 - (1-x)^3}{x} &= \frac{1 - (1 - 3x + 3x^2 - x^3)}{x} \\
&= \frac{3x - 3x^2 + x^3}{x} \\
&= 3 - 3x + x^2
\end{align*}
When $x$ is near zero, there is subtraction of nearly equal numbers.

\item[(c)]
\begin{align*}
\frac{1}{1 + x} - \frac{1}{1 - x} &= \frac{(1 - x) - (1 + x)}{1 - x^2} \\
&= \frac{2x}{x^2 - 1}
\end{align*}
When $x$ is near $\pm1$, there is subtraction of nearly equal numbers.

\end{itemize}

\item 
\[
	x = \frac{-3 \pm \sqrt{9 + 4\times8^{-14}}}{2}
\]
\[
	x_1 = \frac{-3 - \sqrt{9 + 4\times8^{-14}}}{2} = -3
\]
\[
	x_2 = \frac{-3 + \sqrt{9 + 4\times8^{-14}}}{2} = 7.57 \times 10^{-14}
\]
or
\[
	x_2 = \frac{2 \times 8^{-14}}{3 + \sqrt{9 + 4\times8^{-14}}} = 7.58 \times 10^{-14}
\]

\item 
\[
	x_1 = \frac{-b - \sqrt{b^2 + 4 \times 10^{-12}}}{2}
\]
\[
	x_2 = \frac{2 \times 10^{-12}}{-b + \sqrt{b^2 + 4 \times 10^{-12}}}
\]

\item 
\begin{align*}
x_2 &= \frac{-b - \sqrt{b^2 - 4ac}}{2a} \\
&= \frac{(-b - \sqrt{b^2 - 4ac})((-b + \sqrt{b^2 - 4ac}))}{2a((-b + \sqrt{b^2 - 4ac}))} \\
&= \frac{b^2 - (b^2 - 4ac)}{2a((-b + \sqrt{b^2 - 4ac}))} \\
&= \frac{4ac}{2a((-b + \sqrt{b^2 - 4ac}))} \\
&= \frac{2c}{(-b + \sqrt{b^2 - 4ac})} \\
\end{align*}

\end{enumerate}

\end{document}