\documentclass[UTF8]{ctexart}
\usepackage{amsmath}

\begin{document}

\begin{enumerate}
\item \begin{itemize}
\item[(a)] $\frac{1}{4} = 2^{-2} = (1.0 \times 2^{-2})_2$ \\
exponent part: $2^{10} - 1 - 2 = 2^{10} - 3 = (11 \, 1111 \, 1110)_2$ \\
\begin{tabular}{|c|c|c|}
\hline
0011 & 1111 & 1101\\
\hline
\end{tabular} \\
mantissa part: \\
\begin{tabular}{|c|c|c|c|c|c|c|c|c|c|c|c|c|c|c|c|}
\hline
0000 & 0000 & 0000 & 0000 & 0000 & 0000 & 0000 & 0000 & 0000 & 0000 & 0000 & 0000 & 0000\\
\hline
\end{tabular} \\
3FD0 0000 0000 0000
\item[(b)] $\frac{1}{3} = 0.\overline{3333} = (0.\overline{01})_2 = (1.\overline{01} \times 2^{-2})_2$ \\
exponent part: $2^{10} - 1 - 2= 2^{10} - 3 = (11 \, 1111 \, 1110)_2$ \\
\begin{tabular}{|c|c|c|}
\hline
0011 & 1111 & 1101\\
\hline
\end{tabular} \\
mantissa part: \\
\begin{tabular}{|c|c|c|c|c|c|c|c|c|c|c|c|c|c|c|c|}
\hline
0101 & 0101 & 0101 & 0101 & 0101 & 0101 & 0101 & 0101 & 0101 & 0101 & 0101 & 0101 & 0101\\
\hline
\end{tabular} \\
3FD5 5555 5555 5555

\item[ (c) ] $\frac{2}{3} = (0.\overline{10})_2 = (1.\overline{01} \times 2^{-1})_2$ \\
$ \frac{2}{3} \times 2 = \frac{4}{3} = 1 + \frac{1}{3}$ \\
$ \frac{1}{3} \times 2 = \frac{2}{3} $ \\
$ \frac{2}{3} \times 2 = 1 + \frac{1}{3} $ \\
exponent part: $2^{10} - 1 - 1 = (11 1111 1110)_2$ \\
\begin{tabular}{|c|c|c|}
\hline
0011 & 1111 & 1110\\
\hline
\end{tabular} \\
mantissa part: \\
\begin{tabular}{|c|c|c|c|c|c|c|c|c|c|c|c|c|c|c|c|}
\hline
0101 & 0101 & 0101 & 0101 & 0101 & 0101 & 0101 & 0101 & 0101 & 0101 & 0101 & 0101 & 0101\\
\hline
\end{tabular} \\
3FE5 5555 5555 5555

\item[ (d) ] $0.9 = (0.1\overline{1100})_2 = (1.\overline{1100} \times 2^{-1})_2$ \\
$0.9 \times 2 = 1.8 = 1 + 0.8$ \\
$0.8 \times 2 = 1.6 = 1 + 0.6$ \\
$0.6 \times 2 = 1.2 = 1 + 0.2$ \\
$0.2 \times 2 = 0.4$ \\
$0.4 \times 2 = 0.8$ \\
$0.8 \times 2 = 1.6 = 1 + 0.6$ \\
exponent part: $2^{10} - 1 - 1 = (11 1111 1110)_2$ \\
\begin{tabular}{|c|c|c|}
\hline
0011 & 1111 & 1110\\
\hline
\end{tabular} \\
mantissa part: \\
\begin{tabular}{|c|c|c|c|c|c|c|c|c|c|c|c|c|c|c|c|}
\hline
1100&1100&1100&1100&1100&1100&1100&1100&1100&1100&1100&1100&1101\\
\hline
\end{tabular} \\
3FEC CCCC CCCC CCCD

\end{itemize}

\item \begin{itemize}
\item [ (a) ] $9.5 = {1001.1}_2 = (1.0011 \times 2^3)_2$ \\
exponent part: $2^{10} - 1 + 3 = 2^{10} + 2 = (100 0000 0010)_2$ \\
\begin{tabular}{|c|c|c|}
\hline
0100 & 0000 & 0010\\
\hline
\end{tabular} \\
mantissa part: \\
\begin{tabular}{|c|c|c|c|c|c|c|c|c|c|c|c|c|c|c|c|}
\hline
0011&0000&0000&0000&0000&0000&0000&0000&0000&0000&0000&0000&0000\\
\hline
\end{tabular} \\
4023 0000 0000 0000

\item[(b)] $9.6 = (1001.\overline{1001})_2 = (1.001\overline{1001} \times 2^{3})_2$ \\
$0.6 \times 2 = 1.2 = 1 + 0.2$ \\
$0.2 \times 2 = 0.4$ \\
$0.4 \times 2 = 0.8$ \\
$0.8 \times 2 = 1.6 = 1 + 0.6$ \\
$0.6 \times 2 = 1.2 = 1 + 0.2$ \\
exponent part: $2^{10} - 1 + 3 = 2^{10} + 2 = (100 0000 0010)_2$ \\
\begin{tabular}{|c|c|c|}
\hline
0100 & 0000 & 0010\\
\hline
\end{tabular} \\
mantissa part: \\
\begin{tabular}{|c|c|c|c|c|c|c|c|c|c|c|c|c|c|c|c|}
\hline
0011&0011&0011&0011&0011&0011&0011&0011&0011&0011&0011&0011&0011\\
\hline
\end{tabular} \\
4023 3333 3333

\item[(c)] $100.2 = (110 0100.\overline{0011})_2 = (1.100100\overline{0011}\times 2^6)_2$ \\
$0.2 \times 2 = 0.4$ \\
$0.4 \times 2 = 0.8$ \\
$0.8 \times 2 = 1.6 = 1 + 0.6$ \\
$0.6 \times 2 = 1.2 = 1 + 0.2$ \\
exponent part: $2^{10} - 1 + 6 = 2^{10} + 5 = (100 0000 0101)_2$ \\
\begin{tabular}{|c|c|c|}
\hline
0100 & 0000 & 0101\\
\hline
\end{tabular} \\
mantissa part: \\
\begin{tabular}{|c|c|c|c|c|c|c|c|c|c|c|c|c|c|c|c|}
\hline
1001&0000&1100&1100&1100&1100&1100&1100&1100&1100&1100&1100&1101\\
\hline
\end{tabular} \\
4059 0CCC CCCC CCCD

\item[(d)] $\frac{44}{7} = 6 + \frac{2}{7} = (110.0\overline{100})_2 = (1.100\overline{100} \times 2^2)_2$ \\
$\frac{2}{7} \times 2 = \frac{4}{7}$ \\
$\frac{4}{7} \times 2 = 1 + \frac{1}{7}$ \\
$\frac{1}{7} \times 2 = \frac{2}{7}$ \\
$\frac{2}{7} \times 2 = \frac{4}{7}$ \\
$\frac{4}{7} \times 2 = 1 + \frac{1}{7}$ \\
exponent part: $2^{10} - 1 + 2 = 2^{10} + 5 = (100 0000 0001)_2$ \\
\begin{tabular}{|c|c|c|}
\hline
0100 & 0000 & 0001\\
\hline
\end{tabular} \\
mantissa part: \\
\begin{tabular}{|c|c|c|c|c|c|c|c|c|c|c|c|c|c|c|c|}
\hline
1001&0010&0100&1001&0010&0100&1001&0010&0100&1001&0010&0100&1001\\
\hline
\end{tabular} \\
4019 2492 4924 9249

\end{itemize}

\item $5 + 2^{-k} = (101.0 \dots 1 \dots 0)_2 = (1.010 \dots 1 \dots 0 \times 2^2)_2$ \\
$2 + k \le 52$ \\
$k \le 50$

\item $19 + 2^{-k} = (10011.0 \dots 1 \dots)_2 = (1.00110 \dots 1 \dots \times 2^4)_2$ \\
$4 + k \le 52$, $k = 48$

\item \begin{itemize}
\item[(a)] $(1 + (2^{-51} + 2^{-53})) - 1 = 2^{-51}$ \\
$2^{-51} = (0.0000\;0000\;0000\;0000\;0000\;0000\;0000\;0000\;0000\;0000\;0000\;0000\;0010)_2$ \\
$2^{-53} = (0.0000\;0000\;0000\;0000\;0000\;0000\;0000\;0000\;0000\;0000\;0000\;0000\;0000\;1)_2$ \\
\begin{align*}
 &0.0000\;0000\;0000\;0000\;0000\;0000\;0000\;0000\;0000\;0000\;0000\;0000\;0010 \\
+&0.0000\;0000\;0000\;0000\;0000\;0000\;0000\;0000\;0000\;0000\;0000\;0000\;0000\;1 \\
\hline
=&0.0000\;0000\;0000\;0000\;0000\;0000\;0000\;0000\;0000\;0000\;0000\;0000\;0010\;1 
\end{align*}
using the Rounding to Nearest Rule:
\begin{align*}
2^{-51} + 2^{-53} &= (0.0000\;0000\;0000\;0000\;0000\;0000\;0000\;0000\;0000\;0000\;0000\;0000\;0010\;1)_2 \\
                  &= (1.01 \times 2^{-51})_2
\end{align*}
\begin{align*}
 &1.0000\;0000\;0000\;0000\;0000\;0000\;0000\;0000\;0000\;0000\;0000\;0000\;0000 \\
+&0.0000\;0000\;0000\;0000\;0000\;0000\;0000\;0000\;0000\;0000\;0000\;0000\;0010\;1 \\
\hline
=&1.0000\;0000\;0000\;0000\;0000\;0000\;0000\;0000\;0000\;0000\;0000\;0000\;0010\;1 \\
=&1.0000\;0000\;0000\;0000\;0000\;0000\;0000\;0000\;0000\;0000\;0000\;0000\;0010
\end{align*}

\item[(b)] $(1 + (2^{-51} + 2^{-52} + 2^{-53})) - 1 = 2^{-50}$ \\
$2^{-51} = (0.0000\;0000\;0000\;0000\;0000\;0000\;0000\;0000\;0000\;0000\;0000\;0000\;0010)_2$ \\
$2^{-52} = (0.0000\;0000\;0000\;0000\;0000\;0000\;0000\;0000\;0000\;0000\;0000\;0000\;0001)_2$ \\
$2^{-53} = (0.0000\;0000\;0000\;0000\;0000\;0000\;0000\;0000\;0000\;0000\;0000\;0000\;0000\;1)_2$ \\
\begin{align*}
 &0.0000\;0000\;0000\;0000\;0000\;0000\;0000\;0000\;0000\;0000\;0000\;0000\;0010 \\
+&0.0000\;0000\;0000\;0000\;0000\;0000\;0000\;0000\;0000\;0000\;0000\;0000\;0001 \\
\hline
=&0.0000\;0000\;0000\;0000\;0000\;0000\;0000\;0000\;0000\;0000\;0000\;0000\;0011 
\end{align*}
\begin{align*}
 &0.0000\;0000\;0000\;0000\;0000\;0000\;0000\;0000\;0000\;0000\;0000\;0000\;0011 \\
+&0.0000\;0000\;0000\;0000\;0000\;0000\;0000\;0000\;0000\;0000\;0000\;0000\;0000\;1 \\
\hline
=&0.0000\;0000\;0000\;0000\;0000\;0000\;0000\;0000\;0000\;0000\;0000\;0000\;0011\;1 
\end{align*}

\begin{align*}
 &0.0000\;0000\;0000\;0000\;0000\;0000\;0000\;0000\;0000\;0000\;0000\;0000\;0011\;1 \\
+&1.0000\;0000\;0000\;0000\;0000\;0000\;0000\;0000\;0000\;0000\;0000\;0000\;0000 \\
\hline
=&1.0000\;0000\;0000\;0000\;0000\;0000\;0000\;0000\;0000\;0000\;0000\;0000\;0011\;1 \\
=&1.0000\;0000\;0000\;0000\;0000\;0000\;0000\;0000\;0000\;0000\;0000\;0000\;0100 \\
\end{align*}

\end{itemize}

\item \begin{itemize}
\item[(a)] $(1 + (2^{-51} + 2^{-52} + 2^{-54})) - 1 = (1.1 \times 2^{-51})_2$ \\
$2^{-51} = (0.0000\;0000\;0000\;0000\;0000\;0000\;0000\;0000\;0000\;0000\;0000\;0000\;0010)_2$ \\
$2^{-52} = (0.0000\;0000\;0000\;0000\;0000\;0000\;0000\;0000\;0000\;0000\;0000\;0000\;0001)_2$ \\
$2^{-54} = (0.0000\;0000\;0000\;0000\;0000\;0000\;0000\;0000\;0000\;0000\;0000\;0000\;0000\;01)_2$ \\
$2^{-51} + 2^{-52} + 2^{-54} = (0.0000\;0000\;0000\;0000\;0000\;0000\;0000\;0000\;0000\;0000\;0000\;0000\;0011\;01)_2$
\begin{align*}
 &0.0000\;0000\;0000\;0000\;0000\;0000\;0000\;0000\;0000\;0000\;0000\;0000\;0011\;01 \\
+&1.0000\;0000\;0000\;0000\;0000\;0000\;0000\;0000\;0000\;0000\;0000\;0000\;0000 \\
\hline
=&1.0000\;0000\;0000\;0000\;0000\;0000\;0000\;0000\;0000\;0000\;0000\;0000\;0011\;01 \\
=&1.0000\;0000\;0000\;0000\;0000\;0000\;0000\;0000\;0000\;0000\;0000\;0000\;0011 \\
\end{align*}


\item[(b)] $(1 + (2^{-51} + 2^{-52} + 2^{-60})) - 1 = (1.1 \times 2^{-51})_2$ \\
$2^{-51} = (0.0000\;0000\;0000\;0000\;0000\;0000\;0000\;0000\;0000\;0000\;0000\;0000\;0010)_2$ \\
$2^{-52} = (0.0000\;0000\;0000\;0000\;0000\;0000\;0000\;0000\;0000\;0000\;0000\;0000\;0001)_2$ \\
$2^{-60} = (0.0000\;0000\;0000\;0000\;0000\;0000\;0000\;0000\;0000\;0000\;0000\;0000\;0000\;0000\;0001)_2$ \\
\begin{align*}
2^{-51} + 2^{-52} + 2^{-60} = &(0.0000\;0000\;0000\;0000\;0000\;0000\;0000\;0000\;0000\;0000\;0000\;0000\;0011 \\
                              &   0000\;0001)_2
\end{align*}

\begin{align*}
&1 + 2^{-51} + 2^{-52} + 2^{-60} \\
&=(1.0000\;0000\;0000\;0000\;0000\;0000\;0000\;0000\;0000\;0000\;0000\;0000\;0011\;0000\;0001)_2 \\
&=(1.0000\;0000\;0000\;0000\;0000\;0000\;0000\;0000\;0000\;0000\;0000\;0000\;0011)_2
\end{align*}

\end{itemize}

\item \begin{itemize}
\item[(a)] $8 = (1000.0)_2 = (1.0000 \times 2^3)_2 = 4020\;0000\;0000\;0000$
\item[(b)] $21 = 16 + 5 = (1\;0101.000)_2 = (1.0101000 \times 2^4) = 4035\;0000\;0000\;0000$
\item[(c)] $1/8 = 2^{-3} = 3FC0\;0000\;0000\;0000$
\item[(d)] $1/3 = (0.\overline{01})_2 = (1.\overline{01} \times 2^{-2})_2 = 3FD5\;5555\;5555\;5555$ \\
$2 \times \frac{1}{3} = \frac{2}{3}$ \\
$2 \times \frac{2}{3} = 1 + \frac{1}{3}$ \\
$2 \times \frac{1}{3} = \frac{2}{3}$
\item[(e)] $2/3 = 3FE5\;5555\;5555\;5555$
\item[(f)] $0.1 = (0.0\overline{0011})_2 = (1.1\overline{0011} \times 2^{-4})_2 = 3FB9\;9999\;9999\;999A$ \\
$2 \times 0.1 = 0.2$ \\
$2 \times 0.2 = 0.4$ \\
$2 \times 0.4 = 0.8$ \\
$2 \times 0.8 = 1 + 0.6$ \\
$2 \times 0.6 = 1 + 0.2$ \\
$2 \times 0.2 = 0.4$
\item[(g)] $-0.1 = BFB9\;9999\;9999\;999A$
\item[(h)] $-0.2 = -(0.\overline{0011})_2 = -(1.1\overline{0011} \times 2^{-3})_2 = BFC9\;9999\;9999\;999A $ \\
$2 \times 0.2 = 0.4$ \\
$2 \times 0.4 = 0.8$ \\
$2 \times 0.8 = 1 + 0.6$ \\
$2 \times 0.6 = 1 + 0.2$ \\
$2 \times 0.2 = 0.4$

\end{itemize}

\item \begin{itemize}
\item Rounding to Nearest Rule \\
\begin{align*}
\frac{1}{3} &= (1.0101\;0101\;0101\;0101\;0101\;0101\;0101\;0101\;0101\;0101\;0101\;0101\;0101 \times 2^{-2})_2 \\
&=(0.0101\;0101\;0101\;0101\;0101\;0101\;0101\;0101\;0101\;0101\;0101\;0101\;0101\;01)_2
\end{align*}
\begin{align*}
\frac{2}{3} &= (0.\overline{10})_2 = (1.\overline{01} \times 2^{-1})_2 \\
&=(0.1010\;1010\;1010\;1010\;1010\;1010\;1010\;1010\;1010\;1010\;1010\;1010\;1010\;1)_2
\end{align*}
\begin{align*}
 &0.0101\;0101\;0101\;0101\;0101\;0101\;0101\;0101\;0101\;0101\;0101\;0101\;0101\;01 \\
+&0.1010\;1010\;1010\;1010\;1010\;1010\;1010\;1010\;1010\;1010\;1010\;1010\;1010\;1 \\
\hline
=&0.1111\;1111\;1111\;1111\;1111\;1111\;1111\;1111\;1111\;1111\;1111\;1111\;1111\;11 \\
=&1.0000\;0000\;0000\;0000\;0000\;0000\;0000\;0000\;0000\;0000\;0000\;0000\;0000 \\
\end{align*}
\item Chopping result: \\
$0.1111\;1111\;1111\;1111\;1111\;1111\;1111\;1111\;1111\;1111\;1111\;1111\;1111$
\end{itemize}

\item \begin{itemize}
\item[(a)] \begin{align*}
\frac{7}{3} &= 2 + \frac{1}{3} = (10.\overline{01})_2 \\
&= (1.0010\;1010\;1010\;1010\;1010\;1010\;1010\;1010\;1010\;1010\;1010\;1010\;1011 \times 2^1)_2 \\
&=(10.0101\;0101\;0101\;0101\;0101\;0101\;0101\;0101\;0101\;0101\;0101\;0101\;0110)_2
\end{align*}
\begin{align*}
\frac{4}{3} &= 1 + \frac{1}{3} = (1.\overline{01})_2 \\
&= (1.0101\;0101\;0101\;0101\;0101\;0101\;0101\;0101\;0101\;0101\;0101\;0101\;0101)_2
\end{align*}
\begin{align*}
 &10.0101\;0101\;0101\;0101\;0101\;0101\;0101\;0101\;0101\;0101\;0101\;0101\;0110 \\
-&01.0101\;0101\;0101\;0101\;0101\;0101\;0101\;0101\;0101\;0101\;0101\;0101\;0101 \\
\hline
=&01.0000\;0000\;0000\;0000\;0000\;0000\;0000\;0000\;0000\;0000\;0000\;0000\;0001
\end{align*}

\begin{align*}
 &1.0000\;0000\;0000\;0000\;0000\;0000\;0000\;0000\;0000\;0000\;0000\;0000\;0001 \\
-&1.0000\;0000\;0000\;0000\;0000\;0000\;0000\;0000\;0000\;0000\;0000\;0000\;0000 \\
\hline
=&0.0000\;0000\;0000\;0000\;0000\;0000\;0000\;0000\;0000\;0000\;0000\;0000\;0001
\end{align*}
$\epsilon_{mach}$ is introduced when converting $7/3$ to floating point numbers.

\item[(b)] 
$\frac{4}{3} = 1 + \frac{1}{3} = (1.\overline{01})_2$ 
\begin{align*}
\frac{1}{3} &= (0.\overline{01})_2 \\
&= (1.0101\;0101\;0101\;0101\;0101\;0101\;0101\;0101\;0101\;0101\;0101\;0101\;0101 \times 2^{-2})_2
\end{align*}
\begin{align*}
 &1.0101\;0101\;0101\;0101\;0101\;0101\;0101\;0101\;0101\;0101\;0101\;0101\;0101 \\
-&0.0101\;0101\;0101\;0101\;0101\;0101\;0101\;0101\;0101\;0101\;0101\;0101\;0101 \\
\hline
=&1.0000\;0000\;0000\;0000\;0000\;0000\;0000\;0000\;0000\;0000\;0000\;0000\;0000
\end{align*}

\end{itemize}

\item \begin{itemize}
\item[(a)]
\begin{align*}
 &1.0000\;0000\;0000\;0000\;0000\;0000\;0000\;0000\;0000\;0000\;0000\;0000\;0000 \\
+&0.0000\;0000\;0000\;0000\;0000\;0000\;0000\;0000\;0000\;0000\;0000\;0000\;0000\;1 \\
\hline
=&1.0000\;0000\;0000\;0000\;0000\;0000\;0000\;0000\;0000\;0000\;0000\;0000\;0000\;1 \\
=&1.0000\;0000\;0000\;0000\;0000\;0000\;0000\;0000\;0000\;0000\;0000\;0000\;0000
\end{align*}
$1 + 2^{-53} = 1$

\item[(b)]
\begin{align*}
 &0.0000\;0000\;0000\;0000\;0000\;0000\;0000\;0000\;0000\;0000\;0000\;0000\;0000\;1 \\
+&0.0000\;0000\;0000\;0000\;0000\;0000\;0000\;0000\;0000\;0000\;0000\;0000\;0000\;\dots 1 \\
\hline
=&0.0000\;0000\;0000\;0000\;0000\;0000\;0000\;0000\;0000\;0000\;0000\;0000\;0000\;1\dots 1 \\
=&0.0000\;0000\;0000\;0000\;0000\;0000\;0000\;0000\;0000\;0000\;0000\;0000\;0001
\end{align*}
\begin{align*}
 &1.0000\;0000\;0000\;0000\;0000\;0000\;0000\;0000\;0000\;0000\;0000\;0000\;0000 \\
+&0.0000\;0000\;0000\;0000\;0000\;0000\;0000\;0000\;0000\;0000\;0000\;0000\;0001 \\
\hline
=&1.0000\;0000\;0000\;0000\;0000\;0000\;0000\;0000\;0000\;0000\;0000\;0000\;0001
\end{align*}
$1 + (2^{-53} + 2^{-60}) > 1$
\end{itemize}

\item associative law fails.
\item \begin{itemize}
\item[(a)] 
\begin{align*}
\frac{1}{3} &= (0.\overline{01})_2 \\
&= (1.0101\;0101\;0101\;0101\;0101\;0101\;0101\;0101\;0101\;0101\;0101\;0101\;0101 \times 2^{-2})_2
\end{align*}
discarding the infinit tail $0.\overline{01} \times 2^{-53} \times 2^{-2} = 0.000\overline{01} \times 2^{-52}$ \\
\[
	\frac{|fl(1/3) - 1/3|}{1/3} = \frac{0.000\overline{01} \times 2^{-52}}{1/3} = \frac{3}{32} \times 2^{-52} < \epsilon_{mach}/2
\]
\item[(b)]
\begin{align*}
2 \times 0.3 &= 0.6 \\
2 \times 0.6 &= 1.2 = 1 + 0.2 \\
2 \times 0.2 &= 0.4 \\
2 \times 0.4 &= 0.8 \\
2 \times 0.8 &= 1.6 = 1 + 0.6 \\
2 \times 0.6 &= 1.2 = 1 + 0.2
\end{align*}
\begin{align*}
3.3 &= (11.01\overline{0011})_2 \\
&= (1.101\overline{0011} \times 2^{1})_2 \\
&= (1.1010\;0110\;0110\;0110\;0110\;0110\;0110\;0110\;0110\;0110\;0110\;0110\;0110 \times 2^1)_2
\end{align*}
discarding the infinit tail $0.\overline{0110} \times 2^{-53} \times 2^1$
\[
	\frac{|fl(3.3) - 3.3|}{3.3} = \frac{0.\overline{0110} \times 2^{-52}}{3.3} = \frac{0.4}{3.3} \times 2^{-52} < \epsilon_{mach}/2
\]

\item[(c)] $x = \frac{9}{7} = 1 + \frac{2}{7}$
\begin{align*}
2 \times \frac{2}{7} &= \frac{4}{7} \\
2 \times \frac{4}{7} &= \frac{8}{7} = 1 + \frac{1}{7} \\
2 \times \frac{1}{7} &= \frac{2}{7} \\
2 \times \frac{2}{7} &= \frac{4}{7} \\
\end{align*}
\begin{align*}
\frac{9}{7} &= (1.\overline{010})_2 \\
&= (1.0100\;1001\;0010\;0100\;1001\;0010\;0100\;1001\;0010\;0100\;1001\;0010\;0100)_2
\end{align*}
discarding the infinit tail $0.\overline{010} \times 2^{-53}$
\[
	\frac{|fl(9/7) - 9/7|}{9/7} = \frac{0.0\overline{010} \times 2^{-52}}{9/7} = \frac{7}{72} \times 2^{-52} < \epsilon_{mach}/2
\]

\end{itemize}

\item \begin{itemize}
\item[(a)] $(0100\;0000\;0000\;0000\;0000\;0000\;0000\;0000\;0000\;0000\;0000\;0000\;0000\;0000\;0000\;0000)_2$
$2^{10} - (2^{10} - 1) = 1$ \\
the largest number is 2.
\item[(b)] $(0000\;0000\;0000\;1000\;0000\;\dots\;0000)_2 = (1.1)_2 \times 2^{0 - (2^{10} - 1)} = (1.1)_2 \times 2^{-1023}$
\[
(0010\;0000\;0000\;0000\;\dots\;0000)_2 = 2^{2^9 - (2^{10} - 1)} = 2^{-511}
\]

\item[(c)] $(1000\;1000\;\dots\;0000)_2 = 0$
\end{itemize}

\item \begin{itemize}
\item[(a)] $(4.3 - 3.3) - 1$ \\
\begin{align*}
4.3 &= (100.01\overline{0011})_2 \\
&= (1.0001\overline{0011} \times 2^2)_2 \\
&= (1.0001\;0011\;\dots\;0011 \times 2^2)_2
\end{align*}
\begin{align*}
3.3 &= (11.01\overline{0011})_2 \\
&= (1.101\overline{0011} \times 2^1)_2 \\
&= (1.1010\;0110\;0110\;0110\;\dots\;0110\;0110 \times 2^1)_2
\end{align*}

\begin{align*}
 &100.0100\;1100\;1100\;1100\;1100\;1100\;1100\;1100\;1100\;1100\;1100\;1100\;00 \\
-&011.0100\;1100\;1100\;1100\;1100\;1100\;1100\;1100\;1100\;1100\;1100\;1100\;0 \\
\hline
=&001.0000\;0000\;0000\;0000\;0000\;0000\;0000\;0000\;0000\;0000\;0000\;0000
\end{align*}

\item[(b)] $(4.4 - 3.4) - 1$
\begin{align*}
4.4 &= (100.\overline{0110})_2 \\
&= (1.00\overline{0110} \times 2^2)_2 \\
&= (1.0001\;1001\;1001\;1001\;1001\;1001\;1001\;1001\;1001\;1001\;1001\;1001\;1001 \times 2^2)_2 \\
&= (1.0001\;1001\;1001\;1001\;1001\;1001\;1001\;1001\;1001\;1001\;1001\;1010 \times 2^2)_2 \\
\end{align*}
\begin{align*}
3.4 &= (11.\overline{0110})_2 \\
&= (1.1\overline{0110} \times 2^1)_2 \\
&= (1.1011\;0011\;0011\;0011\;0011\;0011\;0011\;0011\;0011\;0011\;0011\;0011\;0011 \times 2^1)_2 \\
&= (1.1011\;0011\;0011\;0011\;0011\;0011\;0011\;0011\;0011\;0011\;0011\;0011 \times 2^1)_2
\end{align*}

\begin{align*}
 &100.0110\;0110\;0110\;0110\;0110\;0110\;0110\;0110\;0110\;0110\;0110\;1000 \\
-&011.0110\;0110\;0110\;0110\;0110\;0110\;0110\;0110\;0110\;0110\;0110\;0110 \\
\hline
=&001.0000\;0000\;0000\;0000\;0000\;0000\;0000\;0000\;0000\;0000\;0000\;0010
\end{align*}
the result is $(0.0000\;0000\;0000\;0000\;0000\;0000\;0000\;0000\;0000\;0000\;0000\;0010)_2 = 2^{-51} = 3CC0\;0000\;0000\;0000$

\item[(c)] $(4.9 - 3.9) - 1$
\begin{align*}
4.9 &= (100.1\overline{1100})_2 \\
&= (1.001\overline{1100} \times 2^2)_2 \\
&= (1.0011\;1001\;1001\;1001\;1001\;1001\;1001\;1001\;1001\;1001\;1001\;1001\;1001\times 2^2)_2 \\
&= (1.0011\;1001\;1001\;1001\;1001\;1001\;1001\;1001\;1001\;1001\;1001\;1010 \times 2^2)_2
\end{align*}
\begin{align*}
3.9 &= (11.1\overline{1100})_2  \\
&= (1.11\overline{1100} \times 2^1)_2 \\
&= (1.1111\;0011\;0011\;0011\;0011\;0011\;0011\;0011\;0011\;0011\;0011\;0011\;0011 \times 2^1)_2 \\
&= (1.1111\;0011\;0011\;0011\;0011\;0011\;0011\;0011\;0011\;0011\;0011\;0011 \times 2^1)_2
\end{align*}
\begin{align*}
 &100.1110\;0110\;0110\;0110\;0110\;0110\;0110\;0110\;0110\;0110\;0110\;1000 \\
-&011.1110\;0110\;0110\;0110\;0110\;0110\;0110\;0110\;0110\;0110\;0110\;0110 \\
\hline
=&001.0000\;0000\;0000\;0000\;0000\;0000\;0000\;0000\;0000\;0000\;0000\;0010
\end{align*}
the result is $(0.0000\;0000\;0000\;0000\;0000\;0000\;0000\;0000\;0000\;0000\;0000\;0010)_2 = 2^{-51} = 3CC0\;0000\;0000\;0000$

\end{itemize}

\item \begin{itemize}
\item[(a)] $(8.3 - 7.3) - 1$
\begin{align*}
8.3 &= (1000.01\overline{0011})_2 \\
&= (1.00001\overline{0011} \times 2^3)_2 \\
&= (1.0000\;1001\;1001\;1001\;1001\;1001\;1001\;1001\;1001\;1001\;1001\;1001\;1001 \times 2^3)_2 \\
&= (1.0000\;1001\;1001\;1001\;1001\;1001\;1001\;1001\;1001\;1001\;1001\;1010 \times 2^3)_2
\end{align*}
\begin{align*}
7.3 &= (111.01\overline{0011})_2 \\
&= (1.1101\overline{0011} \times 2^2)_2 \\
&= (1.1101\;0011\;\dots\;0011\;0011 \times 2^2)_2 \\
&= (1.1101\;0011\;\dots\;0011 \times 2^2)_2
\end{align*}
\begin{align*}
 &1000.0100\;1100\;1100\;1100\;1100\;1100\;1100\;1100\;1100\;1100\;1101\;0000 \\
-&0111.0100\;1100\;1100\;1100\;1100\;1100\;1100\;1100\;1100\;1100\;1100\;1100 \\
\hline
=&0001.0000\;0000\;0000\;0000\;0000\;0000\;0000\;0000\;0000\;0000\;0000\;0100
\end{align*}
the result is $2^{-50} = 3CD0\;0000\;0000\;0000$

\item[(b)] $(8.4 - 7.4) - 1$
\begin{align*}
8.4 &= (1000.\overline{0110})_2 \\
&= (1.000\overline{0110} \times 2^3)_2 \\
&= (1.0000\;1100\;1100\;1100\;1100\;1100\;1100\;1100\;1100\;1100\;1100\;1100\;1100 \times 2^3)_2 \\
&= (1.0000\;1100\;1100\;1100\;1100\;1100\;1100\;1100\;1100\;1100\;1100\;1101 \times 2^3)_2
\end{align*}
\begin{align*}
7.4 &= (111.\overline{0110})_2 \\
&= (1.11\overline{0110} \times 2^2)_2 \\
&= (1.1101\;1001\;1001\;1001\;1001\;1001\;1001\;1001\;1001\;1001\;1001\;1001\;1001 \times 2^2)_2 \\
&= (1.1101\;1001\;1001\;1001\;1001\;1001\;1001\;1001\;1001\;1001\;1001\;1010 \times 2^2)_2
\end{align*}
\begin{align*}
 &1000.0110\;0110\;0110\;0110\;0110\;0110\;0110\;0110\;0110\;0110\;0110\;1000 \\
-&0111.0110\;0110\;0110\;0110\;0110\;0110\;0110\;0110\;0110\;0110\;0110\;1000 \\
\hline
=&0001.0000\;0000\;0000\;0000\;0000\;0000\;0000\;0000\;0000\;0000\;0000\;0000
\end{align*}
the result is zero.

\item[(c)] $(8.8 - 7.8) - 1$
\begin{align*}
8.8 &= (1000.\overline{1100})_2 \\
&= (1.000\overline{1100} \times 2^3)_2 \\
&= (1.0001\;1001\;1001\;1001\;1001\;1001\;1001\;1001\;1001\;1001\;1001\;1001\;1001 \times 2^3)_2 \\
&= (1.0001\;1001\;1001\;1001\;1001\;1001\;1001\;1001\;1001\;1001\;1001\;1010 \times 2^3)_2 \\
\end{align*}
\begin{align*}
7.8 &= (111.\overline{1100})_2 \\
&= (1.11\overline{1100} \times 2^2)_2 \\
&= (1.1111\;0011\;0011\;0011\;0011\;0011\;0011\;0011\;0011\;0011\;0011\;0011\;0011 \times 2^2)_2 \\
&= (1.1111\;0011\;0011\;0011\;0011\;0011\;0011\;0011\;0011\;0011\;0011\;0011 \times 2^2)_2
\end{align*}
\begin{align*}
 &1000.1100\;1100\;1100\;1100\;1100\;1100\;1100\;1100\;1100\;1100\;1101\;0000 \\
-&0111.1100\;1100\;1100\;1100\;1100\;1100\;1100\;1100\;1100\;1100\;1100\;1100 \\
\hline
=&0001.0000\;0000\;0000\;0000\;0000\;0000\;0000\;0000\;0000\;0000\;0000\;0100
\end{align*}
the result is $2^{-50} = 3CD0\;0000\;0000\;0000$

\end{itemize}

\item \begin{itemize}
\item[(a)] $2.75 = (10.11)_2 = (1.011 \times 2)_2$ \\
$fl(2.75) - 2.75 = 0$ \\
\[
	\frac{fl(2.75) - 2.75}{|2.75|} = 0  < \epsilon_{mach}/2
\]
\item[(b)] \begin{align*}
2.7 &= (10.1\overline{0110})_2 \\
&= (1.01\overline{0110} \times 2^1)_2 \\
&= (1.0101\;1001\;1001\;1001\;1001\;1001\;1001\;1001\;1001\;1001\;1001\;1001\;1001 \times 2^1)_2 \\
&= (1.0101\;1001\;1001\;1001\;1001\;1001\;1001\;1001\;1001\;1001\;1001\;1010 \times 2^1)_2
\end{align*}
\begin{align*}
fl(2.7) - 2.7 &= 2^{-52} \times 2^1 - (0.1001)_2 \times 2^{-52} \times 2^1 \\
&= (0.111)_2 \times 2^{-52}
\end{align*}
\[
	\frac{fl(2.7) - 2.7}{2.7} = \frac{(0.111)_2 \times 2^{-52}}{2.7} < \epsilon_{mach}/2
\]
\item[(c)] \begin{align*}
10/3 &= 3 + 1/3 = (11.\overline{01})_2 \\
&= (11.0101\;0101\;0101\;0101\;0101\;0101\;0101\;0101\;0101\;0101\;0101\;0101\;0101\;)_2 \\
&= (1.1010\;1010\;1010\;1010\;1010\;1010\;1010\;1010\;1010\;1010\;1010\;1010\;1010 \times 2^1)_2 \\
&= (1.1010\;1010\;1010\;1010\;1010\;1010\;1010\;1010\;1010\;1010\;1010\;1011 \times 2^1)_2 
\end{align*}
$fl(10/3) - 10/3 = 2^{-52} \times 2^1 - (0.\overline{10})_2 \times 2^{-52} \times 2^1 = 2^{-51}$ \\
\[
	\frac{fl(10/3) - 10/3}{10/3} = 0.3 \times 2^{-52} < \epsilon_{mach}/2 
\]
\end{itemize}

\end{enumerate}
\end{document}