\documentclass[UTF8]{ctexart}
\usepackage{amsmath}

\title{solutions to Exercises 1.2}

\begin{document}
\maketitle

\begin{enumerate}
\item \begin{itemize}
\item[(a)] $\frac{3}{x}$
\begin{gather*}
\frac{3}{x} = x\\
x^2 = 3 \\
x = \pm\sqrt{3}
\end{gather*}

\item[(b)] $x^2 - 2x + 2$
\begin{gather*}
x^2 - 2x + 2 = x \\
x^2 - 3x + 2 = 0 \\
(x - 1)(x - 2) = 0 \\
x = 1 \; \text{or} \;x = 2
\end{gather*}

\item[(c)] $x^2 - 4x + 2$
\begin{gather*}
x^2 - 4x + 2 = x \\
x^2 - 5x + 2 = 0 \\
(-5)^2 - 4 \times 2 = 17 \\
x = \frac{5 \pm \sqrt{17}}{2}
\end{gather*}

\end{itemize}

\item \begin{itemize}
\item[(a)] $\frac{x + 6}{3x - 2}$
\begin{gather*}
\frac{x + 6}{3x - 2} = x \\
x + 6 = 3x^2 - 2x \\
3x^2 - 3x - 6 = 0 \\
x^2 - x - 2 = 0 \\
(x - 2)(x + 1) = 0 \\
x = 2 \; \text{or} \; x = -1
\end{gather*}

\item[(b)] $\frac{8 + 2x}{2 + x^2}$
\begin{gather*}
\frac{8 + 2x}{2 + x^2} = x \\
8 + 2x = 2x + 2x^2 \\
x^2 = 4 \\
x = \pm 2
\end{gather*}

\item[(c)] $x^5$
\begin{gather*}
x^5 = x \\
x^4 = 1 \\
x = \pm 1
\end{gather*}

\end{itemize}

\item \begin{itemize}
\item[(a)]
\[
\frac{x^3 + x - 6}{6x - 10}
\]

\[
\frac{1 + 1 - 6}{6 - 10} = \frac{-4}{-4} = 1
\]

\[
\frac{2^3 + 2 - 6}{6\times2 - 10} = \frac{4}{2} = 2
\]

\[
\frac{3^3 + 3 - 6}{6\times3 - 10} = \frac{24}{8} = 3
\]

\item[(b)]
\[
	\frac{6 + 6x^2 - x^3}{11}
\]

\[
	\frac{6 + 6 - 1}{11} = 1
\]

\[
	\frac{6 + 6 \times 2^2 - 2^3}{11} = 2
\]

\[
	\frac{6 + 6 \times 3^2 - 3^3}{11} = 3
\]

\end{itemize}

\item \begin{itemize}
\item[(a)]
\[
	\frac{4x}{x^2 + 3}
\]

\[
	\frac{-4}{1 + 3} = -1
\]

\[
	\frac{0}{3} = 0
\]

\[
	\frac{4}{1 + 3} = 1
\]

\item[(b)]
\[
	\frac{x^2 - 5x}{x^2 + x - 6}
\]

\[
	\frac{1 + 5}{1 - 1 - 6} = -1
\]

\[
	\frac{0}{-6} = 0
\]

\[
	\frac{1 - 5}{1 + 1 - 6} = 1
\]

\end{itemize}

\item \begin{itemize}
\item[(a)]
\[
	\frac{x}{\sqrt{3}} = \frac{\sqrt{3}}{\sqrt{3}} = 1 \ne \sqrt{3}
\]
$\sqrt{3}$ is not a fixed point.

\item[(b)]
\[
	\frac{2x}{3} + \frac{1}{x} = \frac{2\sqrt{3}}{3} + \frac{1}{\sqrt{3}} = \sqrt{3}
\]
$\sqrt{3}$ is a fixed point.

\item[(c)]
\[
	x^2 - x = 3 - \sqrt{3} \ne = \sqrt{3}
\]
$\sqrt{3}$ is not a fixed point.

\item[(d)]
\[
	1 + \frac{2}{x + 1} = 1 + \frac{2}{\sqrt{3} + 1} = 1 + \frac{2(\sqrt{3} - 1)}{(\sqrt{3} + 1)(\sqrt{3} - 1)} = \sqrt{3}
\]
$\sqrt{3}$ is a fixed point.

\end{itemize}

\item \begin{itemize}
\item[(a)]
\[
	\frac{5 + 7x}{x + 7} = \frac{5 + 7\sqrt{5}}{\sqrt{5} + 7} = \frac{(5 + 7\sqrt{5}}{(\sqrt{5} + 7)\sqrt{5}}\sqrt{5} = \sqrt{5}
\]
$\sqrt{5}$ is a fixed point.

\item[(b)]
\[
	\frac{10}{3x} + \frac{x}{3} = \frac{10}{3\sqrt{5}} + \frac{\sqrt{5}}{3} = \frac{10\sqrt{5}}{3 \times 5} + \frac{\sqrt{5}}{3} = \sqrt{5}
\]
$\sqrt{5}$ is a fixed point.

\item[(c)]
\[
	x^2 - 5 = 0
\]
$\sqrt{5}$ is not a fixed point.

\item[(d)]
\[
	1 + \frac{4}{x + 1} = 1 + \frac{4}{\sqrt{5} + 1} = \sqrt{5}
\]
$\sqrt{5}$ is a fixed point.

\end{itemize}

\item 
\begin{itemize}
\item[(a)]
\begin{gather*}
g(x) = (2x - 1)^{1/3} \\
g'(x) = \frac{2}{3}(2x - 1)^{-2/3} \\
g'(1) = 0 < 1
\end{gather*}
Fixed-Point Iteration is locally convergent to the given fixed point $r=1$.

\item[(b)]
\begin{gather*}
g(x) = \frac{x^3 + 1}{2} \\
g'(x) = \frac{3}{2}x^2 \\
g'(1) = \frac{3}{2} > 1
\end{gather*}
Fixed-Point Iteration is not locally convergent to the given fixed point $r=1$.

\item[(c)]
\begin{gather*}
g(x) = \sin x + x \\
g'(x) = \cos x + 1 \\
g'(0) = 2 > 1
\end{gather*}
Fixed-Point Iteration is not locally convergent to the given fixed point $r=0$.

\end{itemize}

\item \begin{itemize}
\item[(a)]
\begin{gather*}
g(x) = \frac{2x - 1}{x^2} = \frac{2}{x} - \frac{1}{x^2} \\
g'(x) = -2x^{-2} + 2x^{-3} \\
g'(1) = 0 < 1
\end{gather*}
Fixed-Point Iteration is locally convergent to the given fixed point $r=1$.

\item[(b)]
\begin{gather*}
g(x) = \cos x + \pi + 1 \\
g'(x) = -\sin x \\
g'(\pi) = 0
\end{gather*}
Fixed-Point Iteration is locally convergent to the given fixed point $r=\pi$.

\item[(c)]
\begin{gather*}
g(x) = e^{2x} - 1 \\
g'(x) = 2e^{2x} \\
g'(x) = 2 > 1
\end{gather*}
Fixed-Point Iteration is not locally convergent to the given fixed point $r=0$.

\end{itemize}

\item \begin{itemize}
\item[(a)]
\begin{gather*}
	g(x) = \frac{1}{2}x^2 + \frac{1}{2}x \\
	\frac{1}{2}x^2 + \frac{1}{2}x = x \\
	\frac{1}{2}x^2 - \frac{1}{2}x = 0 \\
	x = 0 \; \text{or} \; x = 1
\end{gather*}

\begin{gather*}
g'(x) = x + \frac{1}{2}
\end{gather*}

If $x = 0$, $g'(0) = \frac{1}{2} < 1$, Fixed-Point Iteration of $g(x)$ is locally convergent to it. \\
If $x = 1$, $g'(\frac{1}{2}) = \frac{3}{2} > 1$, Fixed-Point Iteration of $g(x)$ is not locally convergent to it.

\item[(b)]
\begin{gather*}
g(x) = x^2 - \frac{1}{4}x + \frac{3}{8} \\
x^2 - \frac{1}{4}x + \frac{3}{8} = x \\
x^2 - \frac{5}{4}x + \frac{3}{8} = 0 \\
8x^2 - 10x + 3 = 0 \\
x = \frac{10 \pm \sqrt{100 - 4 \times 8 \times 3}}{16} \\
x = \frac{3}{4} \; \text{or} \; x = \frac{1}{2}
\end{gather*}

\begin{gather*}
g'(x) = 2x - \frac{1}{4}
\end{gather*}

If $x = \frac{3}{4}$, $g'(\frac{3}{4}) = \frac{5}{4} > 1$, Fixed-Point Iteration of $g(x)$ is not locally convergent to it.\\
If $x = \frac{1}{2}$, $g'(\frac{1}{2}) = \frac{3}{4} < 1$, Fixed-Point Iteration of $g(x)$ is locally convergent to it.

\end{itemize}

\item \begin{itemize}
\item[(a)]
\begin{gather*}
x^2 - \frac{3}{2}x + \frac{3}{2} = x \\
x^2 - \frac{5}{2}x + \frac{3}{2} = 0 \\
2x^2 - 5x + 3 = 0 \\
(x - 1)(2x - 3) = 0 \\
x = 1 \; \text{or} \; x = \frac{3}{2}
\end{gather*}

\begin{gather*}
g'(x) = 2x - \frac{3}{2}x
\end{gather*}

If $x = 1$, $g'(1) = \frac{1}{2} < 1$, Fixed-Point Iteration of $g(x)$ is locally convergent to it.\\
If $x = \frac{3}{2}$, $g'(\frac{3}{2}) = 2\frac{3}{2} - \frac{3}{2}\frac{3}{2} = 3 - \frac{9}{4} = \frac{3}{4} < 1$, Fixed-Point Iteration of $g(x)$ is locally convergent to it.

\item[(b)]
\begin{gather*}
x^2 + \frac{1}{2}x - \frac{1}{2} = x \\
x^2 - \frac{1}{2}x - \frac{1}{2} = 0 \\
2x^2 - x - 1 = 0 \\
(x - 1)(2x + 1) = 0 \\
x = 1 \; \text{or} \; x = -\frac{1}{2}
\end{gather*}

\[
	g'(x) = 2x + \frac{1}{2}
\]

If $x = 1$, $g'(1) = 2 + \frac{1}{2} > 1$, Fixed-Point Iteration of $g(x)$ is not locally convergent to it. \\
If $x = -\frac{1}{2}$, $|g'(-\frac{1}{2})| = \frac{1}{2} < 1$, Fixed-Point Iteration of $g(x)$ is locally convergent to it.
\end{itemize}

\item \begin{itemize}
\item[(a)] 
\[
	x^3 - x + e^x = 0
\]
\begin{gather*}
x^3 + e^x = x \\
\sqrt[3]{x - e^x} = x \\
\ln{(x - x^3)} = x
\end{gather*}

\item[(b)]
\[
	3x^{-2} + 9x^3 = x^2
\]
\begin{gather*}
3 + 9x^5 = x^4 \\
\sqrt[5]{\frac{x^4 - 3}{9}} = x \\
3x^{-2} + 9x^3 - x^2 + x = x \\
x^2 - 3x^{-2} = 9x^3 \\
\sqrt[3]{\frac{x^2 - 3x^{-2}}{9}} = x
\end{gather*}

\end{itemize}

\item \begin{itemize}
\item[(a)]
\begin{gather*}
g(x) = x^2 - 0.24 \\
g'(x) = 2x \\
g'(0.2) = 0.4 < 0.5
\end{gather*}
Fixed-Point Iteration is locally convergent to $r = 0.2$, it is faster than the Bisection Method.

\item[(b)]
\begin{gather*}
x^2 - 0.24 = x \\
x^2 - x - 0.24 = 0 \\
(x - 1.2)(x + 0.2) = 0 \\
x = 1.2 \; \text{or} \; x = -0.2
\end{gather*}

If $x = 1.2$, $g'(1.2) = 1.2^2 - 0.24 = 1.2 > 1$, Fixed-Point Iteration is not locally convergent to $r = 1.2$,

\end{itemize}

\item \begin{itemize}
\item[(a)] 
\begin{gather*}
0.39 - x^2 = x \\
x^2 + x - 0.39 = 0 \\
(x - 0.3)(x + 1.3) = 0 \\
x = 0.3 \; \text{or} \; x = -1.3
\end{gather*}

\item[(b)]
\[
	g'(x) = -2x
\]
If $x = 0.3$, $|g'(0.3)| = |-0.6| < 1$, FPI converge to it. \\
If $x = -1.3$, $|g'(1.3)| > 1$, FPI does't converge to it.

\item[(c)]
Because $|g'(0.3)| > 0.5$, FPI converge to this fixed point slower than the Bisection Method.

\end{itemize}

\item \begin{itemize}
\item[(A)]
\begin{gather*}
g(x) = \frac{1}{2}x + \frac{1}{x} \\
g'(x) = \frac{1}{2} - \frac{1}{x^2} \\
g'(\sqrt{2}) = 0 < 1
\end{gather*}

\item[(B)]
\begin{gather*}
g(x) = \frac{2}{3}x + \frac{2}{3x} \\
g'(x) = \frac{2}{3} - \frac{2}{3x^2} \\
g'(\sqrt{2}) = \frac{1}{3} < 1
\end{gather*}

\item[(C)]
\begin{gather*}
g(x) = \frac{3}{4}x + \frac{1}{2x} \\
g'(x) = \frac{3}{4} - \frac{1}{2x^2} \\
g'(\sqrt{2}) = \frac{1}{2} < 1
\end{gather*}

\end{itemize}

Rank: $A > B > C$

\item \begin{itemize}
\item[(A)]
\begin{gather*}
g(x) = \frac{4}{5}x + \frac{1}{x} \\
g'(x) = \frac{4}{5} - \frac{1}{x^2} \\
g'(\sqrt{5}) = \frac{4}{5} - \frac{1}{5} = \frac{3}{5} = 0.6 < 1
\end{gather*}

\item[(B)]
\begin{gather*}
g(x) = \frac{x}{2} + \frac{5}{2x} \\
g'(x) = \frac{1}{2} - \frac{5}{2x^2} \\
g'(\sqrt{5}) = \frac{1}{2} - \frac{5}{10} = 0 < 1
\end{gather*}

\item[(C)]
\begin{gather*}
g(x) = \frac{x+5}{x+1} \\
g'(x) = \frac{x+1 - (x+5)}{(x+1)^2} = \frac{-4}{(x+1)^2} \\
|g'(\sqrt{5})| = \frac{4}{(\sqrt{5} + 1)^2} = 0.382 < 1
\end{gather*}

\end{itemize}
Rank $B > C > A$

\item \begin{itemize}
\item[(A)] 
\begin{gather*}
g(x) = \frac{2}{\sqrt{x}} \\
|g'(x)| = |2 \times (-\frac{1}{2}) x^{-3/2}| = |-x^{-3/2}| \\
|g'(\sqrt[3]{4})| = \frac{1}{\sqrt{4}} = \frac{1}{2} < 1
\end{gather*}

\item[(B)]
\begin{gather*}
g(x) = \frac{3x}{4} + \frac{1}{x^2} \\
g'(x) = \frac{3}{4} - \frac{2}{x^3} \\
g'(x) = \frac{3}{4} - \frac{2}{4} = \frac{1}{4} < 1
\end{gather*}

\item[(C)]
\begin{gather*}
g(x) = \frac{2x}{3} + \frac{4}{3x^2} \\
g'(x) = \frac{2}{3} - \frac{8}{3x^3} \\
g'(x) = \frac{2}{3} - \frac{8}{12} = 0 < 1
\end{gather*}

\end{itemize}

Rank: $C > B > A$

\item 
\begin{gather*}
	g(x) = 2x^2 + x - 1 \\
	g(1/2) = \frac{1}{2} + \frac{1}{2} - 1 = 0 \\
	g(-1) = 2 - 1 - 1 = 0
\end{gather*}

\begin{gather*}
	2x^2 + x - 1 = 0\\
	x^2 = \frac{1 - x}{2} \\
	f_1(x) = \sqrt{\frac{1 - x}{2}} = \frac{1}{\sqrt{2}}(1 - x)^{1/2} \\
	f_2(x) = -\sqrt{\frac{1 - x}{2}} = -\frac{1}{\sqrt{2}}(1 - x)^{1/2} \\
	f_1'(x) = \frac{1}{2\sqrt{2}} \times (1 - x)^{-1/2} \times (-1) = -\frac{1}{2\sqrt{2}} (1 - x)^{-1/2} \\
	f_2'(x) = -\frac{1}{2\sqrt{2}} \times (1 - x)^{-1/2} \times (-1) = \frac{1}{2\sqrt{2}} (1 - x)^{-1/2} \\
	|f_1'(1/2)| = \frac{1}{2\sqrt{2}} (\frac{1}{2})^{-1/2} = \frac{1}{2} < 1\\
	|f_2'(-1)| = \frac{1}{2\sqrt{2}} (\frac{1}{2})^{-1/2} = \frac{1}{2} < 1
\end{gather*}

\item Suppose $k$ is an integer, and $k > 1$,
\begin{gather*}
	x^2 = k \\
	x = \frac{k}{x} \\
	2x = x + \frac{k}{x} \\
	\frac{1}{2}(x + \frac{k}{x}) = x \\
	g(x) = \frac{1}{2}(x + \frac{k}{x}) \\
	g'(x) = \frac{1}{2}(1 - \frac{k}{x^2})
\end{gather*}

if $x^2 = k - 1$, 
\[
	|g'(x)| = |\frac{1}{2}(1 - \frac{k}{k - 1})| = |\frac{1}{2(k-1)}| < 1
\]

if $x^2 = k + 1$,
\[
	|g'(x)| = |\frac{1}{2}(1 - \frac{k}{k + 1})| = |\frac{1}{2(k+1)}| < 1
\]

if $k-1 < x^2 < k+1$, $|g'(x)| < 1$

\item 
\begin{gather*}
x^3 = A \\
x = \frac{A}{x^2} \\
2x = x + \frac{A}{x^2} \\
x = \frac{1}{2}(x + \frac{A}{x^2}) \\
g(x) = \frac{1}{2}(x + \frac{A}{x^2}) \\
g'(x) = \frac{1}{2}(1 - \frac{2A}{x^3})
\end{gather*}

\item

\item

\item

\item

\end{enumerate}

\end{document}